wip on lamda-DOT, which is, even though it has no self
references nor recursion, more challenging than expected

dev/existential/lambda-DOT.v
@@ -468,6 +468,10 @@ with subtyp: ctx -> typ -> typ -> Prop :=
   | subtyp_or_r: forall G S T1 T2,
       subtyp G S T2 ->
       subtyp G S (typ_or T1 T2)
+  | subtyp_trans: forall G T1 T2 T3,
+      subtyp G T1 T2 ->
+      subtyp G T2 T3 ->
+      subtyp G T1 T3
 with subdec: ctx -> dec -> dec -> Prop :=
   | subdec_typ: forall G L Lo1 Hi1 Lo2 Hi2,
       (* Lo2 <: Lo1 <: Hi1 <: Hi2 *)
@@ -482,6 +486,8 @@ with subdec: ctx -> dec -> dec -> Prop :=
       subtyp G S2 S1 ->
       subtyp G T1 T2 ->
       subdec G (dec_mtd m S1 T1) (dec_mtd m S2 T2)
+  | subdec_refl: forall G D,
+      subdec G D D
 with ty_trm: ctx -> trm -> typ -> Prop :=
   | ty_var: forall G x T,
       binds x T G ->
@@ -551,3 +557,1488 @@ Inductive wf_sto: sto -> ctx -> Prop :=
       ty_defs G ds T ->
       (* No need to check if realizable bounds, because that's already done by ty_def *)
       wf_sto (s & x ~ ds) (G & x ~ T).
+
+
+(* ###################################################################### *)
+(** ** Statements we want to prove *)
+
+Definition progress := forall s G e T,
+  wf_sto s G ->
+  ty_trm G e T -> 
+  (
+    (* can step *)
+    (exists e' s', red e s e' s') \/
+    (* or is a value *)
+    (exists x o, e = (trm_var (avar_f x)) /\ binds x o s)
+  ).
+
+Definition preservation := forall s G e T e' s',
+  wf_sto s G -> ty_trm G e T -> red e s e' s' ->
+  (exists G', wf_sto s' G' /\ ty_trm G' e' T).
+
+
+(* ###################################################################### *)
+(* ###################################################################### *)
+(** * Infrastructure *)
+
+(* ###################################################################### *)
+(** ** Induction principles *)
+
+Scheme trm_mut  := Induction for trm  Sort Prop
+with   def_mut  := Induction for def  Sort Prop
+with   defs_mut := Induction for defs Sort Prop.
+Combined Scheme trm_mutind from trm_mut, def_mut, defs_mut.
+
+Scheme typ_mut  := Induction for typ  Sort Prop
+with   dec_mut  := Induction for dec  Sort Prop.
+Combined Scheme typ_mutind from typ_mut, dec_mut.
+
+Scheme typ_has_mut := Induction for typ_has Sort Prop
+with   subtyp_mut  := Induction for subtyp  Sort Prop
+with   subdec_mut  := Induction for subdec  Sort Prop
+with   ty_trm_mut  := Induction for ty_trm  Sort Prop
+with   ty_def_mut  := Induction for ty_def  Sort Prop
+with   ty_defs_mut := Induction for ty_defs Sort Prop
+with   can_add_mut := Induction for can_add Sort Prop.
+Combined Scheme ty_mutind from typ_has_mut,
+                               subtyp_mut, subdec_mut,
+                               ty_trm_mut, ty_def_mut, ty_defs_mut, can_add_mut.
+
+Scheme subtyp_mut2  := Induction for subtyp  Sort Prop
+with   subdec_mut2  := Induction for subdec  Sort Prop.
+Combined Scheme subtyp_subdec_mut from subtyp_mut2, subdec_mut2.
+
+
+(* ###################################################################### *)
+(** ** Tactics *)
+
+Ltac gather_vars :=
+  let A := gather_vars_with (fun x : vars      => x         ) in
+  let B := gather_vars_with (fun x : var       => \{ x }    ) in
+  let C := gather_vars_with (fun x : ctx       => (dom x) \u (fv_ctx_types x)) in
+  let D := gather_vars_with (fun x : sto       => dom x     ) in
+  let E := gather_vars_with (fun x : avar      => fv_avar  x) in
+  let F := gather_vars_with (fun x : trm       => fv_trm   x) in
+  let G := gather_vars_with (fun x : def       => fv_def   x) in
+  let H := gather_vars_with (fun x : defs      => fv_defs  x) in
+  let I := gather_vars_with (fun x : typ       => fv_typ   x) in
+  let J := gather_vars_with (fun x : dec       => fv_dec   x) in
+  constr:(A \u B \u C \u D \u E \u F \u G \u H \u I \u J).
+
+Ltac pick_fresh x :=
+  let L := gather_vars in (pick_fresh_gen L x).
+
+Tactic Notation "apply_fresh" constr(T) "as" ident(x) :=
+  apply_fresh_base T gather_vars x.
+
+Hint Constructors typ_has subtyp subdec ty_trm ty_def ty_defs can_add.
+Hint Constructors defs_has defs_hasnt.
+
+Lemma fresh_push_eq_inv: forall A x a (E: env A),
+  x # (E & x ~ a) -> False.
+Proof.
+  intros. rewrite dom_push in H. false H. rewrite in_union.
+  left. rewrite in_singleton. reflexivity.
+Qed.
+
+
+(* ###################################################################### *)
+(** ** Definition of var-by-var substitution *)
+
+(** Note that substitution is not part of the definitions, because for the
+    definitions, opening is sufficient. For the proofs, however, we also
+    need substitution, but only var-by-var substitution, not var-by-term
+    substitution. That's why we don't need a judgment asserting that a term
+    is locally closed. *)
+
+Definition subst_avar (z: var) (u: var) (a: avar) : avar :=
+  match a with
+  | avar_b i => avar_b i
+  | avar_f x => If x = z then (avar_f u) else (avar_f x)
+  end.
+
+Definition subst_pth (z: var) (u: var) (p: pth) : pth :=
+  match p with
+  | pth_var a => pth_var (subst_avar z u a)
+  end.
+
+Fixpoint subst_typ (z: var) (u: var) (T: typ) { struct T } : typ :=
+  match T with
+  | typ_top     => typ_top
+  | typ_bot     => typ_bot
+  | typ_rcd D   => typ_rcd (subst_dec z u D)
+  | typ_sel p L => typ_sel (subst_pth z u p) L
+  | typ_and T1 T2 => typ_and (subst_typ z u T1) (subst_typ z u T2)
+  | typ_or  T1 T2 => typ_or  (subst_typ z u T1) (subst_typ z u T2)
+  end
+with subst_dec (z: var) (u: var) (D: dec) { struct D } : dec :=
+  match D with
+  | dec_typ L T U => dec_typ L (subst_typ z u T) (subst_typ z u U)
+  | dec_fld l T   => dec_fld l (subst_typ z u T)
+  | dec_mtd m T U => dec_mtd m (subst_typ z u T) (subst_typ z u U)
+  end.
+
+Fixpoint subst_trm (z: var) (u: var) (t: trm) : trm :=
+  match t with
+  | trm_var x        => trm_var (subst_avar z u x)
+  | trm_new ds       => trm_new (subst_defs z u ds)
+  | trm_sel t l      => trm_sel (subst_trm z u t) l
+  | trm_call t1 m t2 => trm_call (subst_trm z u t1) m (subst_trm z u t2)
+  end
+with subst_def (z: var) (u: var) (d: def) : def :=
+  match d with
+  | def_typ L T1 T2   => def_typ L (subst_typ z u T1) (subst_typ z u T2)
+  | def_fld l T x     => def_fld l (subst_typ z u T) (subst_avar z u x)
+  | def_mtd m T1 T2 b => def_mtd m (subst_typ z u T1) (subst_typ z u T2) (subst_trm z u b)
+  end
+with subst_defs (z: var) (u: var) (ds: defs) : defs :=
+  match ds with
+  | defs_nil => defs_nil
+  | defs_cons rest d => defs_cons (subst_defs z u rest) (subst_def z u d)
+  end.
+
+Definition subst_ctx (z: var) (u: var) (G: ctx) : ctx := map (subst_typ z u) G.
+
+
+(* ###################################################################### *)
+(** ** Lemmas for var-by-var substitution *)
+
+Lemma subst_fresh_avar: forall x y,
+  (forall a: avar, x \notin fv_avar a -> subst_avar x y a = a).
+Proof.
+  intros. destruct* a. simpl. case_var*. simpls. notin_false.
+Qed.
+
+Lemma subst_fresh_pth: forall x y,
+  (forall p: pth, x \notin fv_pth p -> subst_pth x y p = p).
+Proof.
+  intros. destruct p. simpl. f_equal. apply* subst_fresh_avar.
+Qed.
+
+Lemma subst_fresh_typ_dec_decs: forall x y,
+  (forall T : typ , x \notin fv_typ  T  -> subst_typ  x y T  = T ) /\
+  (forall d : dec , x \notin fv_dec  d  -> subst_dec  x y d  = d ).
+Proof.
+  intros x y. apply typ_mutind; intros; simpls; f_equal*. apply* subst_fresh_pth.
+Qed.
+
+Definition subst_fresh_typ(x y: var) := proj1 (subst_fresh_typ_dec_decs x y).
+
+Lemma subst_fresh_trm_def_defs: forall x y,
+  (forall t : trm , x \notin fv_trm  t  -> subst_trm  x y t  = t ) /\
+  (forall d : def , x \notin fv_def  d  -> subst_def  x y d  = d ) /\
+  (forall ds: defs, x \notin fv_defs ds -> subst_defs x y ds = ds).
+Proof.
+  intros x y. apply trm_mutind; intros; simpls; f_equal*;
+    (apply* subst_fresh_avar || apply* subst_fresh_typ_dec_decs).
+Qed.
+
+Lemma invert_fv_ctx_types_push: forall x z T G,
+  x \notin fv_ctx_types (G & z ~ T) -> x \notin fv_typ T /\ x \notin (fv_ctx_types G).
+Proof.
+  introv N.
+  unfold fv_ctx_types in *.
+  unfold fv_in_values in *.
+  rewrite <- cons_to_push in *.
+  rewrite values_def in *.
+  unfold LibList.map in *.
+  do 2 rewrite LibList.fold_right_cons in *.
+  simpl in *.
+  apply notin_union in N. exact N.
+Qed.
+
+Lemma subst_fresh_ctx: forall x y G,
+  x \notin fv_ctx_types G -> subst_ctx x y G = G.
+Proof.
+  intros x y.
+  apply (env_ind (fun G => x \notin fv_ctx_types G -> subst_ctx x y G = G)).
+  + intro N. unfold subst_ctx. apply map_empty.
+  + intros G z T IH N.
+    apply invert_fv_ctx_types_push in N. destruct N as [N1 N2].
+    unfold subst_ctx in *. rewrite map_push.
+    rewrite (IH N2).
+    rewrite (subst_fresh_typ _ _ N1).
+    reflexivity.
+Qed.
+
+Definition subst_fvar(x y z: var): var := If x = z then y else z.
+
+Lemma subst_open_commute_avar: forall x y u,
+  (forall a: avar, forall n: Datatypes.nat,
+    subst_avar x y (open_rec_avar n u a) 
+    = open_rec_avar n (subst_fvar x y u) (subst_avar  x y a)).
+Proof.
+  intros. unfold subst_fvar, subst_avar, open_avar, open_rec_avar. destruct a.
+  + repeat case_if; auto.
+  + case_var*.
+Qed.
+
+Lemma subst_open_commute_pth: forall x y u,
+  (forall p: pth, forall n: Datatypes.nat,
+    subst_pth x y (open_rec_pth n u p) 
+    = open_rec_pth n (subst_fvar x y u) (subst_pth x y p)).
+Proof.
+  intros. unfold subst_pth, open_pth, open_rec_pth. destruct p.
+  f_equal. apply subst_open_commute_avar.
+Qed.
+
+(* "open and then substitute" = "substitute and then open" *)
+Lemma subst_open_commute_typ_dec_decs: forall x y u,
+  (forall t : typ, forall n: Datatypes.nat,
+     subst_typ x y (open_rec_typ n u t)
+     = open_rec_typ n (subst_fvar x y u) (subst_typ x y t)) /\
+  (forall d : dec , forall n: Datatypes.nat, 
+     subst_dec x y (open_rec_dec n u d)
+     = open_rec_dec n (subst_fvar x y u) (subst_dec x y d)).
+Proof.
+  intros. apply typ_mutind; intros; simpl; f_equal*. apply subst_open_commute_pth.
+Qed.
+
+(* "open and then substitute" = "substitute and then open" *)
+Lemma subst_open_commute_trm_def_defs: forall x y u,
+  (forall t : trm, forall n: Datatypes.nat,
+     subst_trm x y (open_rec_trm n u t)
+     = open_rec_trm n (subst_fvar x y u) (subst_trm x y t)) /\
+  (forall d : def , forall n: Datatypes.nat, 
+     subst_def x y (open_rec_def n u d)
+     = open_rec_def n (subst_fvar x y u) (subst_def x y d)) /\
+  (forall ds: defs, forall n: Datatypes.nat, 
+     subst_defs x y (open_rec_defs n u ds)
+     = open_rec_defs n (subst_fvar x y u) (subst_defs x y ds)).
+Proof.
+  intros. apply trm_mutind; intros; simpl; f_equal*;
+    (apply* subst_open_commute_avar || apply* subst_open_commute_typ_dec_decs).
+Qed.
+
+Lemma subst_open_commute_trm: forall x y u t,
+  subst_trm x y (open_trm u t) = open_trm (subst_fvar x y u) (subst_trm x y t).
+Proof.
+  intros. apply* subst_open_commute_trm_def_defs.
+Qed.
+
+Lemma subst_open_commute_defs: forall x y u ds,
+  subst_defs x y (open_defs u ds) = open_defs (subst_fvar x y u) (subst_defs x y ds).
+Proof.
+  intros. apply* subst_open_commute_trm_def_defs.
+Qed.
+
+Lemma subst_open_commute_typ: forall x y u T,
+  subst_typ x y (open_typ u T) = open_typ (subst_fvar x y u) (subst_typ x y T).
+Proof.
+  intros. apply* subst_open_commute_typ_dec_decs.
+Qed.
+
+Lemma subst_open_commute_dec: forall x y u D,
+  subst_dec x y (open_dec u D) = open_dec (subst_fvar x y u) (subst_dec x y D).
+Proof.
+  intros. apply* subst_open_commute_typ_dec_decs.
+Qed.
+
+(* "Introduce a substitution after open": Opening a term t with a var u is the
+   same as opening t with x and then replacing x by u. *)
+Lemma subst_intro_trm: forall x u t, x \notin (fv_trm t) ->
+  open_trm u t = subst_trm x u (open_trm x t).
+Proof.
+  introv Fr. unfold open_trm. rewrite* subst_open_commute_trm.
+  destruct (@subst_fresh_trm_def_defs x u) as [Q _]. rewrite* (Q t).
+  unfold subst_fvar. case_var*.
+Qed.
+
+Lemma subst_intro_defs: forall x u ds, x \notin (fv_defs ds) ->
+  open_defs u ds = subst_defs x u (open_defs x ds).
+Proof.
+  introv Fr. unfold open_trm. rewrite* subst_open_commute_defs.
+  destruct (@subst_fresh_trm_def_defs x u) as [_ [_ Q]]. rewrite* (Q ds).
+  unfold subst_fvar. case_var*.
+Qed.
+
+Lemma subst_intro_typ: forall x u T, x \notin (fv_typ T) ->
+  open_typ u T = subst_typ x u (open_typ x T).
+Proof.
+  introv Fr. unfold open_typ. rewrite* subst_open_commute_typ.
+  destruct (@subst_fresh_typ_dec_decs x u) as [Q _]. rewrite* (Q T).
+  unfold subst_fvar. case_var*.
+Qed.
+
+Lemma subst_intro_dec: forall x u D, x \notin (fv_dec D) ->
+  open_dec u D = subst_dec x u (open_dec x D).
+Proof.
+  introv Fr. unfold open_trm. rewrite* subst_open_commute_dec.
+  destruct (@subst_fresh_typ_dec_decs x u) as [_ Q]. rewrite* (Q D).
+  unfold subst_fvar. case_var*.
+Qed.
+
+Lemma subst_undo_avar: forall x y,
+  (forall a, y \notin fv_avar a -> (subst_avar y x (subst_avar x y a)) = a).
+Proof.
+  intros. unfold subst_avar, subst_fvar, open_avar, open_rec_avar; destruct a.
+  + reflexivity.
+  + unfold fv_avar in H. assert (y <> v) by auto. repeat case_if; reflexivity.
+Qed.
+
+Lemma subst_undo_pth: forall x y,
+  (forall p, y \notin fv_pth p -> (subst_pth y x (subst_pth x y p)) = p).
+Proof.
+  intros. destruct p. unfold subst_pth. f_equal.
+  unfold fv_pth in H.
+  apply* subst_undo_avar.
+Qed.
+
+Lemma subst_undo_typ_dec_decs: forall x y,
+   (forall T , y \notin fv_typ  T  -> (subst_typ  y x (subst_typ  x y T )) = T )
+/\ (forall D , y \notin fv_dec  D  -> (subst_dec  y x (subst_dec  x y D )) = D ).
+Proof.
+  intros.
+  apply typ_mutind; intros; simpl; unfold fv_typ, fv_dec in *; f_equal*.
+  apply* subst_undo_pth.
+Qed.
+
+Lemma subst_undo_trm_def_defs: forall x y,
+   (forall t , y \notin fv_trm  t  -> (subst_trm  y x (subst_trm  x y t )) = t )
+/\ (forall d , y \notin fv_def  d  -> (subst_def  y x (subst_def  x y d )) = d )
+/\ (forall ds, y \notin fv_defs ds -> (subst_defs y x (subst_defs x y ds)) = ds).
+Proof.
+  intros.
+  apply trm_mutind; intros; simpl; unfold fv_trm, fv_def, fv_defs in *; f_equal*;
+    (apply* subst_undo_avar || apply* subst_undo_typ_dec_decs).
+Qed.
+
+Lemma subst_typ_undo: forall x y T,
+  y \notin fv_typ T -> (subst_typ y x (subst_typ x y T)) = T.
+Proof.
+  apply* subst_undo_typ_dec_decs.
+Qed.
+
+Lemma subst_dec_undo: forall x y D,
+  y \notin fv_dec D -> (subst_dec y x (subst_dec x y D)) = D.
+Proof.
+  apply* subst_undo_typ_dec_decs.
+Qed.
+
+Lemma subst_trm_undo: forall x y t,
+  y \notin fv_trm t -> (subst_trm y x (subst_trm x y t)) = t.
+Proof.
+  apply* subst_undo_trm_def_defs.
+Qed.
+
+
+(* ###################################################################### *)
+(** ** Trivial inversion lemmas *)
+
+Lemma invert_subdec_typ_sync_right: forall G D2 L Lo1 Hi1,
+  subdec G (dec_typ L Lo1 Hi1) D2 ->
+  (dec_typ L Lo1 Hi1) = D2 \/
+  exists Lo2 Hi2, D2 = (dec_typ L Lo2 Hi2) /\
+                  subtyp G Lo2 Lo1 /\
+                  subtyp G Lo1 Hi1 /\
+                  subtyp G Hi1 Hi2.
+Proof.
+  introv Sd. inversions Sd.
+  - right. exists Lo2 Hi2. auto.
+  - left. reflexivity.
+Qed.
+
+Lemma invert_subdec_typ_sync_left: forall G D1 L Lo2 Hi2,
+   subdec G D1 (dec_typ L Lo2 Hi2) ->
+   D1 = (dec_typ L Lo2 Hi2) \/
+   exists Lo1 Hi1, D1 = (dec_typ L Lo1 Hi1) /\
+                   subtyp G Lo2 Lo1 /\
+                   subtyp G Lo1 Hi1 /\
+                   subtyp G Hi1 Hi2.
+Proof.
+  introv Sd. inversions Sd.
+  - right. exists Lo1 Hi1. auto.
+  - auto.
+Qed.
+
+Lemma invert_subdec_fld_sync_left: forall G D l T2,
+   subdec G D (dec_fld l T2) ->
+   D = (dec_fld l T2) \/
+   exists T1, D = (dec_fld l T1) /\
+              subtyp G T1 T2.
+Proof.
+  introv Sd. inversions Sd.
+  - right. exists T1. auto.
+  - auto.
+Qed.
+
+Lemma invert_subdec_mtd_sync_left: forall G D m T2 U2,
+   subdec G D (dec_mtd m T2 U2) ->
+   D = (dec_mtd m T2 U2) \/
+   exists T1 U1, D = (dec_mtd m T1 U1) /\
+                 subtyp G T2 T1 /\
+                 subtyp G U1 U2.
+Proof.
+  introv Sd. inversions Sd.
+  - right. exists S1 T1. auto.
+  - auto.
+Qed.
+
+Lemma invert_ty_defs_cons: forall G ds0 T1 T2,
+  ty_defs G ds0 (typ_and T1 T2) ->
+  exists d ds D, ds0 = defs_cons ds d /\
+                 ty_defs G ds T1 /\
+                 T2 = typ_rcd D /\
+                 ty_def G d D.
+Proof.
+  introv H. inversions H. exists d ds D. auto.
+Qed.
+
+Lemma wf_sto_to_ok_s: forall s G,
+  wf_sto s G -> ok s.
+Proof. intros. induction H; jauto. Qed.
+
+Lemma wf_sto_to_ok_G: forall s G,
+  wf_sto s G -> ok G.
+Proof. intros. induction H; jauto. Qed.
+
+Hint Resolve wf_sto_to_ok_s wf_sto_to_ok_G.
+
+Lemma ctx_binds_to_sto_binds: forall s G x T,
+  wf_sto s G ->
+  binds x T G ->
+  exists o, binds x o s.
+Proof.
+  introv Wf Bi. gen x T Bi. induction Wf; intros.
+  + false* binds_empty_inv.
+  + unfolds binds. rewrite get_push in *. case_if.
+    - eauto.
+    - eauto.
+Qed.
+
+Lemma sto_binds_to_ctx_binds: forall s G x ds,
+  wf_sto s G ->
+  binds x ds s ->
+  exists T, binds x T G.
+Proof.
+  introv Wf Bi. gen x Bi. induction Wf; intros.
+  + false* binds_empty_inv.
+  + unfolds binds. rewrite get_push in *. case_if.
+    - inversions Bi. exists T. reflexivity.
+    - auto.
+Qed.
+
+Lemma sto_unbound_to_ctx_unbound: forall s G x,
+  wf_sto s G ->
+  x # s ->
+  x # G.
+Proof.
+  introv Wf Ub_s.
+  induction Wf.
+  + auto.
+  + destruct (classicT (x0 = x)) as [Eq | Ne].
+    - subst. false (fresh_push_eq_inv Ub_s). 
+    - auto.
+Qed.
+
+Lemma ctx_unbound_to_sto_unbound: forall s G x,
+  wf_sto s G ->
+  x # G ->
+  x # s.
+Proof.
+  introv Wf Ub.
+  induction Wf.
+  + auto.
+  + destruct (classicT (x0 = x)) as [Eq | Ne].
+    - subst. false (fresh_push_eq_inv Ub). 
+    - auto.
+Qed.
+
+Lemma invert_ty_var: forall G x T,
+  ty_trm G (trm_var (avar_f x)) T ->
+  exists T', subtyp G T' T /\ binds x T' G.
+Proof.
+  introv Ty. gen_eq t: (trm_var (avar_f x)). gen x.
+  induction Ty; intros x' Eq; try (solve [ discriminate ]).
+  + inversions Eq. exists T.
+    apply (conj (subtyp_refl _ _)). assumption.
+  + subst. specialize (IHTy _ eq_refl). destruct IHTy as [T' [St Bi]].
+    exists T'. split.
+    - apply subtyp_trans with T.
+      * apply St.
+      * apply H.
+    - apply Bi.
+Qed.
+
+
+(* ###################################################################### *)
+(** ** Weakening *)
+
+Lemma weakening:
+   (forall G T D, typ_has G T D -> forall G1 G2 G3,
+      G = G1 & G3 ->
+      ok (G1 & G2 & G3) ->
+      typ_has (G1 & G2 & G3) T D)
+/\ (forall G T1 T2, subtyp G T1 T2 -> forall G1 G2 G3,
+      G = G1 & G3 ->
+      ok (G1 & G2 & G3) ->
+      subtyp (G1 & G2 & G3) T1 T2)
+/\ (forall G D1 D2, subdec G D1 D2 -> forall G1 G2 G3,
+      G = G1 & G3 ->
+      ok (G1 & G2 & G3) ->
+      subdec (G1 & G2 & G3) D1 D2)
+/\ (forall G t T, ty_trm G t T -> forall G1 G2 G3,
+      G = G1 & G3 ->
+      ok (G1 & G2 & G3) ->
+      ty_trm (G1 & G2 & G3) t T)
+/\ (forall G d D, ty_def G d D -> forall G1 G2 G3,
+      G = G1 & G3 ->
+      ok (G1 & G2 & G3) ->
+      ty_def (G1 & G2 & G3) d D)
+/\ (forall G ds Ds, ty_defs G ds Ds -> forall G1 G2 G3,
+      G = G1 & G3 ->
+      ok (G1 & G2 & G3) ->
+      ty_defs (G1 & G2 & G3) ds Ds)
+/\ (forall G ds d, can_add G ds d -> forall G1 G2 G3,
+      G = G1 & G3 ->
+      ok (G1 & G2 & G3) ->
+      can_add (G1 & G2 & G3) ds d).
+Proof.
+  apply ty_mutind.
+  + (* case typ_rcd_has *)
+    intros. apply* typ_rcd_has.
+  + (* case typ_sel_has *)
+    intros. apply* typ_sel_has.
+  + (* case typ_and_has_1 *)
+    intros. apply* typ_and_has_1.
+  + (* case typ_and_has_2 *)
+    intros. apply* typ_and_has_2.
+  + (* case typ_and_has_12 *)
+    intros. apply* typ_and_has_12.
+  + (* case typ_or_has *)
+    intros. apply* typ_or_has.
+  + (* case subtyp_refl *)
+    intros. apply subtyp_refl.
+  + (* case subtyp_top *)
+    intros. apply subtyp_top.
+  + (* case subtyp_bot *)
+    intros. apply subtyp_bot.
+  + (* case subtyp_rcd *)
+    intros. apply* subtyp_rcd.
+  + (* case subtyp_sel_l *)
+    intros. subst. apply* subtyp_sel_l.
+  + (* case subtyp_sel_r *)
+    intros. subst. apply* subtyp_sel_r.
+  + (* case subtyp_and *)
+    intros. apply* subtyp_and.
+  + (* case subtyp_and_l *)
+    intros. apply* subtyp_and_l.
+  + (* case subtyp_and_r *)
+    intros. apply* subtyp_and_r.
+  + (* case subtyp_or *)
+    intros. apply* subtyp_or.
+  + (* case subtyp_or_l *)
+    intros. apply* subtyp_or_l.
+  + (* case subtyp_or_r *)
+    intros. apply* subtyp_or_r.
+  + (* case subtyp_trans *)
+    intros. subst. apply* subtyp_trans.
+  + (* case subdec_typ *)
+    intros. apply* subdec_typ.
+  + (* case subdec_fld *)
+    intros. apply* subdec_fld.
+  + (* case subdec_mtd *)
+    intros. apply* subdec_mtd.
+  + (* case subdec_refl *)
+    intros. apply* subdec_refl.
+  + (* case ty_var *)
+    intros. subst. apply ty_var. apply* binds_weaken.
+  + (* case ty_sel *)
+    intros. subst. apply* ty_sel.
+  + (* case ty_call *)
+    intros. subst. apply* ty_call.
+  + (* case ty_new *)
+    intros G ds T Tyds IHTyds G1 G2 G3 Eq Ok. subst. apply* ty_new.
+  + (* case ty_sbsm *)
+    intros. apply ty_sbsm with T.
+    - apply* H.
+    - apply* H0.
+  + (* case ty_typ *)
+    intros. apply* ty_typ. 
+  + (* case ty_fld *)
+    intros. apply* ty_fld.
+  + (* case ty_mtd *) 
+    intros. subst. rename H into IH.
+    apply_fresh ty_mtd as x.
+    rewrite <- concat_assoc.
+    refine (IH x _ G1 G2 (G3 & x ~ S) _ _).
+    - auto.
+    - symmetry. apply concat_assoc.
+    - rewrite concat_assoc. auto.
+  + (* case ty_dsnil *) 
+    intros. apply ty_dsnil.
+  + (* case ty_dscons *) 
+    intros. apply* ty_dscons.
+  + (* case can_add_typ *)
+    intros. apply* can_add_typ.
+  + (* case can_refine_typ *)
+    intros. apply* can_refine_typ.
+  + (* case can_add_fld *)
+    intros. apply* can_add_fld.
+  + (* case can_add_mtd *)
+    intros. apply* can_add_mtd.
+Qed.
+
+Lemma weaken_subtyp_middle: forall G1 G2 G3 S U,
+  ok (G1 & G2 & G3) -> 
+  subtyp (G1      & G3) S U ->
+  subtyp (G1 & G2 & G3) S U.
+Proof.
+  destruct weakening as [_ [W _]].
+  introv Hok123 Hst.
+  specialize (W (G1 & G3) S U Hst).
+  specialize (W G1 G2 G3 eq_refl Hok123).
+  apply W.
+Qed.
+
+Lemma env_add_empty: forall (P: ctx -> Prop) (G: ctx), P G -> P (G & empty).
+Proof.
+  intros.
+  assert ((G & empty) = G) by apply concat_empty_r.
+  rewrite -> H0. assumption.
+Qed.  
+
+Lemma env_remove_empty: forall (P: ctx -> Prop) (G: ctx), P (G & empty) -> P G.
+Proof.
+  intros.
+  assert ((G & empty) = G) by apply concat_empty_r.
+  rewrite <- H0. assumption.
+Qed.
+
+Lemma weaken_subtyp_end: forall G1 G2 S U,
+  ok (G1 & G2) -> 
+  subtyp G1        S U ->
+  subtyp (G1 & G2) S U.
+Proof.
+  introv Hok Hst.
+  apply (env_remove_empty (fun G0 => subtyp G0 S U) (G1 & G2)).
+  apply weaken_subtyp_middle.
+  apply (env_add_empty (fun G0 => ok G0) (G1 & G2) Hok).
+  apply (env_add_empty (fun G0 => subtyp G0 S U) G1 Hst).
+Qed.
+
+Lemma weaken_subdec_middle: forall G1 G2 G3 S U,
+  ok (G1 & G2 & G3) -> 
+  subdec (G1      & G3) S U ->
+  subdec (G1 & G2 & G3) S U.
+Proof.
+  destruct weakening as [_ [_ [W _]]].
+  introv Hok123 Hst.
+  specialize (W (G1 & G3) S U Hst).
+  specialize (W G1 G2 G3 eq_refl Hok123).
+  apply W.
+Qed.
+
+Lemma weaken_subdec_end: forall G1 G2 D1 D2,
+  ok (G1 & G2) -> 
+  subdec G1        D1 D2 ->
+  subdec (G1 & G2) D1 D2.
+Proof.
+  introv Ok Sd.
+  destruct weakening as [_ [_ [W _]]].
+  rewrite <- (concat_empty_r G1) in Sd.
+  specialize (W (G1 & empty) D1 D2 Sd G1 G2 empty).
+  repeat progress rewrite concat_empty_r in *.
+  apply (W eq_refl Ok).
+Qed.
+
+Lemma weaken_ty_trm_end: forall G1 G2 e T,
+  ok (G1 & G2) -> ty_trm G1 e T -> ty_trm (G1 & G2) e T.
+Proof.
+  intros.
+  destruct weakening as [_ [_ [_ [W _]]]].
+  rewrite <- (concat_empty_r (G1 & G2)).
+  apply (W (G1 & empty)); rewrite* concat_empty_r.
+Qed.
+
+Lemma weaken_ty_defs_end: forall G1 G2 is Ds,
+  ok (G1 & G2) -> ty_defs G1 is Ds -> ty_defs (G1 & G2) is Ds.
+Proof.
+  intros.
+  destruct weakening as [_ [_ [_ [_ [_ [W _]]]]]].
+  rewrite <- (concat_empty_r (G1 & G2)).
+  apply (W (G1 & empty)); rewrite* concat_empty_r.
+Qed.
+
+Lemma weaken_ty_trm_middle: forall G1 G2 G3 t T,
+  ok (G1 & G2 & G3) -> ty_trm (G1 & G3) t T -> ty_trm (G1 & G2 & G3) t T.
+Proof.
+  intros. apply* weakening.
+Qed.
+
+
+(* ###################################################################### *)
+(** ** More inversion lemmas *)
+
+Lemma invert_wf_sto: forall s G,
+  wf_sto s G ->
+    forall x ds T,
+      binds x ds s -> 
+      binds x T G ->
+      exists G1 G2,
+        G = G1 & x ~ T & G2 /\ 
+        ty_defs G ds T.
+Proof.
+  intros s G Wf. induction Wf; intros.
+  + false* binds_empty_inv.
+  + unfold binds in *. rewrite get_push in *.
+    case_if.
+    - inversions H2. inversions H3.
+      exists G (@empty typ). rewrite concat_empty_r.
+      apply (conj eq_refl).
+      lets Ok: (wf_sto_to_ok_G Wf).
+      refine (weaken_ty_defs_end _ H1). auto.
+    - specialize (IHWf x0 ds0 T0 H2 H3).
+      destruct IHWf as [G1 [G2 [EqG Ty]]]. subst.
+      exists G1 (G2 & x ~ T).
+      rewrite concat_assoc.
+      apply (conj eq_refl).
+      apply weaken_ty_defs_end.
+      * apply wf_sto_to_ok_G in Wf. auto.
+      * exact Ty.
+Qed.
+
+Lemma invert_wf_sto_with_sbsm: forall s G,
+  wf_sto s G ->
+  forall x ds T2, 
+    binds x ds s ->
+    ty_trm G (trm_var (avar_f x)) T2 -> (* <- instead of binds *)
+    exists T1, subtyp G T1 T2
+            /\ ty_defs G ds T1.
+Proof.
+  introv Wf Bis Tyx.
+  apply invert_ty_var in Tyx. destruct Tyx as [T' [St BiG]].
+  destruct (invert_wf_sto Wf Bis BiG) as [G1 [G2 [Eq Tyds]]].
+  subst. exists T'.
+  lets Ok: (wf_sto_to_ok_G Wf).
+  apply (conj St).
+  auto.
+Qed.
+
+Lemma invert_wf_sto_without_binds: forall s G x T2,
+  wf_sto s G ->
+  ty_trm G (trm_var (avar_f x)) T2 ->
+  exists T1 ds,
+    ty_defs G ds T1 /\
+    subtyp G T1 T2 /\
+    binds x T1 G /\
+    binds x ds s.
+Proof.
+  introv Wf Ty.
+  apply invert_ty_var in Ty. destruct Ty as [T1 [St BiG]].
+  lets Bis: (ctx_binds_to_sto_binds Wf BiG). destruct Bis as [ds Bis].
+  lets P: (invert_wf_sto Wf Bis BiG). destruct P as [G1 [G2 [Eq Tyds]]].
+  exists T1 ds. apply (conj Tyds). apply (conj St). apply (conj BiG Bis).
+Qed.
+
+
+(* ###################################################################### *)
+(** ** Misc *)
+
+Definition ctx_size(G: ctx) := LibList.length G.
+
+Lemma ctx_size_zero_inv: forall G, ctx_size G = 0 -> G = empty.
+Proof.
+  rewrite empty_def.
+  apply LibList.length_zero_inv.
+Qed.
+
+Lemma vars_dont_type_in_empty_env: forall G t T,
+  ty_trm G t T ->
+  forall x, t = (trm_var (avar_f x)) ->
+  G = empty ->
+  False.
+Proof.
+  introv Ty. induction Ty; try discriminate; intros x' Eq1 Eq2; inversions Eq1.
+  + (* case ty_var *)
+    apply (binds_empty_inv H).
+  + (* case ty_sbsm *)
+    inversions H0. apply* IHTy.
+Qed.
+
+
+(* ###################################################################### *)
+(** ** Soundness helper lemmas *)
+
+(* Hyptheses:  X1 ----subtyp----> X2 ----typ_has---> D2
+   Conclusion: X1 ----typ_has---> D1 ----subdec----> D1
+In the system which used expansion instead of typ_has, this didn't work,
+because we were not sure if X1 had an expansion or not. *)
+Definition swap_sub_and_has_until(n: nat) := forall s G x X1 X2 D2,
+  subtyp G X1 X2 ->
+  typ_has G X2 D2 ->
+  ctx_size G <= n ->
+  wf_sto s G ->
+  ty_trm G (trm_var (avar_f x)) X1 -> (* <-- witnesses realizability of X1 *)
+  exists D1,
+    typ_has G X1 D1 /\
+    subdec G D1 D2.
+
+Lemma swap_sub_and_has_base: swap_sub_and_has_until 0.
+Proof.
+  introv St THas Eq' Wf Ty. assert (Eq: ctx_size G = 0) by omega.
+   apply ctx_size_zero_inv in Eq. subst.
+  exfalso. apply (@vars_dont_type_in_empty_env _ _ _ Ty x eq_refl eq_refl).
+Qed.
+
+(* "widens G T1 T2" means that "G |- T1 <: T2" and T2 does not contain path types,
+    and T2 is the smallest such type.
+Inductive widens: ctx -> typ -> typ -> Prop :=
+| widens_top: forall G,
+    widens G typ_top typ_top
+| widens_bot: forall G,
+    widens G typ_bot typ_bot
+|*)
+
+(* "no_path_types T" means that T contains no path types (but T's members can) *)
+Inductive no_path_types: typ -> Prop :=
+| no_path_types_top: no_path_types typ_top
+| no_path_types_bot: no_path_types typ_bot
+| no_path_types_rcd: forall D, no_path_types (typ_rcd D)
+| no_path_types_and: forall T1 T2,
+    no_path_types T1 -> no_path_types T2 -> no_path_types (typ_and T1 T2)
+| no_path_types_or: forall T1 T2,
+    no_path_types T1 -> no_path_types T2 -> no_path_types (typ_or T1 T2).
+
+Inductive is_bot: ctx -> typ -> Prop :=
+| is_bot_bot: forall G, is_bot G typ_bot
+| is_bot_sel: forall G p T L Lo Hi,
+     ty_trm G (pth2trm p) T ->
+     typ_has G T (dec_typ L Lo Hi) ->
+     is_bot G Hi ->
+     is_bot G (typ_sel p L)
+| is_bot_and_l: forall G T1 T2, is_bot G T1 -> is_bot G (typ_and T1 T2)
+| is_bot_and_r: forall G T1 T2, is_bot G T2 -> is_bot G (typ_and T1 T2)
+| is_bot_or: forall G T1 T2, is_bot G T1 -> is_bot G T2 -> is_bot G (typ_or T1 T2).
+
+Lemma subtyp_preserves_is_bot: forall G T1 T2,
+  subtyp G T1 T2 ->
+  is_bot G T2 ->
+  is_bot G T1.
+Proof.
+  introv St. induction St; intros Ib.
+  + (* case subtyp_refl *)
+    assumption.
+  + (* case subtyp_top *)
+    inversions Ib.
+  + (* case subtyp_bot *)
+    apply is_bot_bot.
+  + (* case subtyp_rcd *)
+    inversions Ib.
+  + (* case subtyp_sel_l *)
+    apply (is_bot_sel _ H H0). apply (IHSt Ib).
+  + (* case subtyp_sel_r *)
+    inversions Ib. apply IHSt2. apply IHSt1. admit. (* TODO imprecision!!!*)
+  + (* case subtyp_and *)
+    inversions Ib; auto.
+  + (* case subtyp_and_l *)
+    apply is_bot_and_l. apply* IHSt.
+  + (* case subtyp_and_r *)
+    apply is_bot_and_r. apply* IHSt.
+  + (* case subtyp_or *)
+    apply is_bot_or; auto.
+  + (* case subtyp_or_l *)
+    inversions Ib; auto.
+  + (* case subtyp_or_r *)
+    inversions Ib; auto.
+  + (* case subtyp_trans *)
+    apply IHSt1. apply IHSt2. exact Ib.
+Qed.
+
+Module V2.
+
+Inductive is_bot: typ -> Prop :=
+| is_bot_bot: is_bot typ_bot
+| is_bot_and_l: forall T1 T2, is_bot T1 -> is_bot (typ_and T1 T2)
+| is_bot_and_r: forall T1 T2, is_bot T2 -> is_bot (typ_and T1 T2)
+| is_bot_or: forall T1 T2, is_bot T1 -> is_bot T2 -> is_bot (typ_or T1 T2).
+
+Lemma subtyp_preserves_is_bot: forall G T1 T2,
+  subtyp G T1 T2 ->
+  is_bot T2 ->
+  (*no_path_types T1 ->*)
+  is_bot T1.
+Proof.
+  introv St. induction St; intros Ib (* N*).
+  + (* case subtyp_refl *)
+    assumption.
+  + (* case subtyp_top *)
+    inversions Ib.
+  + (* case subtyp_bot *)
+    apply is_bot_bot.
+  + (* case subtyp_rcd *)
+    inversions Ib.
+  + (* case subtyp_sel_l *)
+    admit. (*inversions N. TODO............*)
+  + (* case subtyp_sel_r *)
+    inversions Ib.
+  + (* case subtyp_and *)
+    inversions Ib; auto.
+  + (* case subtyp_and_l *)
+    apply is_bot_and_l. apply* IHSt.
+  + (* case subtyp_and_r *)
+    apply is_bot_and_r. apply* IHSt.
+  + (* case subtyp_or *)
+    apply is_bot_or; auto.
+  + (* case subtyp_or_l *)
+    inversions Ib; auto.
+  + (* case subtyp_or_r *)
+    inversions Ib; auto.
+  + (* case subtyp_trans *)
+    apply IHSt1. apply IHSt2. exact Ib.
+Qed.
+
+End V2.
+
+Lemma type_of_defs_contains_no_path_types: forall G ds T,
+  ty_defs G ds T -> no_path_types T.
+Proof.
+  introv Tyds. induction Tyds.
+  + apply no_path_types_top.
+  + apply no_path_types_and.
+    - exact IHTyds.
+    - apply no_path_types_rcd.
+Qed.
+
+(*
+Lemma invert_no_path_type_subtyp_of_bot: forall G T,
+  subtyp G T typ_bot ->
+  no_path_types T ->
+  is_bot T.
+Proof.
+  introv St. gen_eq T': typ_bot. induction St; intros Eq N; subst.
+  + (* case subtyp_refl *)
+    apply is_bot_bot.
+  + (* case subtyp_top *)
+    discriminate.
+  + (* case subtyp_bot *)
+    apply is_bot_bot.
+  + (* case subtyp_rcd *)
+    discriminate.
+  + (* case subtyp_sel_l *)
+    inversions N.
+  + (* case subtyp_sel_r *)
+    discriminate.
+  + (* case subtyp_and *)
+    discriminate.
+  + (* case subtyp_and_l *)
+    inversions N. apply is_bot_and_l. apply* IHSt.
+  + (* case subtyp_and_r *)
+    inversions N. apply is_bot_and_r. apply* IHSt.
+  + (* case subtyp_or *)
+    inversions N. apply is_bot_or; auto.
+  + (* case subtyp_or_l *)
+    discriminate.
+  + (* case subtyp_or_r *)
+    discriminate.
+  + (* case subtyp_trans *)
+    admit.
+*)
+
+Lemma defs_are_not_bot: forall G ds X1,
+  subtyp G X1 typ_bot ->
+  ty_defs G ds X1 ->
+  False.
+Proof.
+  introv St. gen ds. gen_eq X2: typ_bot. induction St; intro Eq; subst.
+  + (* case subtyp_refl *)
+    introv Tyds. inversions Tyds.
+  + (* case subtyp_top *)
+    discriminate.
+  + (* case subtyp_bot *)
+    introv Tyds. inversions Tyds.
+  + (* case subtyp_rcd *)
+    discriminate.
+  + (* case subtyp_sel_l *)
+    introv Tyds. inversions Tyds. (* defs don't type as p.L *)
+  + (* case subtyp_sel_r *)
+    discriminate.
+  + (* case subtyp_and *)
+    discriminate.
+  + (* case subtyp_and_l *)
+    introv Tyds. apply invert_ty_defs_cons in Tyds. rename ds into ds0.
+    destruct Tyds as [d [ds [D [Eq1 [Tyds [Eq2 Tyd]]]]]]. subst. apply* IHSt.
+  + (* case subtyp_and_r *)
+    introv Tyds. apply invert_ty_defs_cons in Tyds. rename ds into ds0.
+    destruct Tyds as [d [ds [D [Eq1 [Tyds [Eq2 Tyd]]]]]]. subst.
+    admit. (* TODO typ_rcd might be a subtype of typ_bot in an unrealizable env! *)
+  + (* case subtyp_or *)
+    introv Tyds. inversions Tyds.
+  + (* case subtyp_or_l *)
+    introv Tyds. discriminate.
+  + (* case subtyp_or_r *)
+    introv Tyds. discriminate.
+  + (* case subtyp_trans *)
+    introv Tyds. refine (IHSt1 _ _ Tyds). (* TODO might not hold!  *)
+Abort.
+
+Lemma defs_are_not_bot: forall s G ds X1 x,
+  subtyp G X1 typ_bot ->
+  ty_defs G ds X1 ->
+  wf_sto s G ->
+  binds x X1 G ->
+  binds x ds s ->
+  False.
+Proof.
+  introv St. gen s ds x. gen_eq X2: typ_bot. induction St; intro Eq; subst.
+  + (* case subtyp_refl *)
+    introv Tyds Wf BiG Bis. inversions Tyds.
+  + (* case subtyp_top *)
+    discriminate.
+  + (* case subtyp_bot *)
+    introv Tyds Wf BiG Bis. inversions Tyds.
+  + (* case subtyp_rcd *)
+    discriminate.
+  + (* case subtyp_sel_l *)
+    introv Tyds Wf BiG Bis. inversions Tyds. (* defs don't type as p.L *)
+  + (* case subtyp_sel_r *)
+    discriminate.
+  + (* case subtyp_and *)
+    discriminate.
+  + (* case subtyp_and_l *)
+    introv Tyds Wf BiG Bis. apply invert_ty_defs_cons in Tyds. rename ds into ds0.
+    destruct Tyds as [d [ds [D [Eq1 [Tyds [Eq2 Tyd]]]]]]. subst. admit. (* apply* IHSt. *)
+  + (* case subtyp_and_r *)
+    admit.
+  + (* case subtyp_or *)
+    admit.
+  + (* case subtyp_or_l *)
+    admit.
+  + (* case subtyp_or_r *)
+    admit.
+  + (* case subtyp_trans *)
+    admit.
+Qed.
+
+(*
+    destruct p as [v]. destruct v as [n|v]; [admit | idtac]. (* cannot have bound var *)
+    inversions Tyds.
+    refine (IHSt eq_refl s _ v _ Wf _ _).
+    apply IHSt.
+*)
+
+Lemma swap_sub_and_has_step: forall n,
+  swap_sub_and_has_until n -> swap_sub_and_has_until (S n).
+Proof.
+  introv swap_sub_and_has_IH. introv St. gen s x D2. induction St.
+  + (* case subtyp_refl *)
+    intros. exists D2. auto.
+  + (* case subtyp_top *)
+    intros. inversions H. (* contradiction *)
+  + (* case subtyp_bot *)
+    introv THas Eq Wf Tyx. rename T into X2.
+    lets P: (invert_wf_sto_without_binds Wf Tyx).
+    destruct P as [X1 [ds [Tyds [St [BiG Bis]]]]].
+ admit. (* TODO need witness that T is not bottom *)
+  + (* case subtyp_rfn_l *)
+    intros G T1 l0 D0 T2 n St IHSt l D2 T2Has.
+    specialize (IHSt _ _ T2Has).
+    destruct IHSt as [D1 [L [n' [T1Has Sd]]]]. exists D1 L n'. split.
+    - apply typ_rfn_has_1. exact T1Has.
+    - intros x xL. specialize (Sd x xL).
+      lets St': (subtyp_tmode (subtyp_rfn_l l0 D0 (subtyp_tmode (subtyp_refl G T1 0)))).
+      refine (narrow_subdec_end _ St' Sd). apply okadmit.
+  + (* case subtyp_rfn_r *)
+    introv St IHSt T1Has Sd T2Has. rename l into ll. rename l0 into l.
+    apply invert_typ_rfn_has in T2Has.
+    destruct T2Has as [T2Has | [[M [Eq1 Eq2]] | [D2' [T2Has [Eq1 Eq2]]]]].
+    - (* T2Has only looked left *)
+      specialize (IHSt _ _ T2Has). destruct IHSt as [D1' [L' [n' [T1Has' Sd']]]].
+      exists D1' L' n'. auto.
+    - (* T2Has only looked right *)
+      subst ll D0. exists D1 L n. auto.
+    - (* T2Has took intersection of left and right *)
+      subst.
+      specialize (IHSt _ _ T2Has). destruct IHSt as [D1' [L' [n' [T1Has' Sd']]]].
+      exists (intersect_dec D1' D1) (L' \u L) (max n' n). split.
+      * apply (intersect_typ_has T1Has' T1Has).
+      * intros x N. 
+        assert (xL: x \notin L) by auto. specialize (Sd x xL).
+        assert (xL': x \notin L') by auto. specialize (Sd' x xL').
+        admit. (* TODO distribute open over intersect etc, should hold *)
+  + (* case subtyp_sel_l *)
+    intros G p L Lo Hi T2 n pHas St IHSt l D2 T2Has.
+    specialize (IHSt _ _ T2Has). destruct IHSt as [D1 [F [n' [HiHas Sd]]]].
+    exists D1 F n'. split.
+    - apply (typ_sel_has p pHas HiHas).
+    - intros x xF. specialize (Sd x xF).
+      lets St': (subtyp_tmode (subtyp_sel_l _ pHas (subtyp_tmode (subtyp_refl _ _ 0)))).
+      refine (narrow_subdec_end _ St' Sd). apply okadmit.
+  + (* case subtyp_sel_r *)
+    intros G p L Lo1 Hi1 T1 n pHas1 St1 IH1 St2 IH2 l D2 pLHas.
+    apply invert_typ_sel_has in pLHas. destruct pLHas as [Lo2 [Hi2 [pHas2 Hi2Has]]].
+    lets P: (intersect_has pHas1 pHas2). simpl in P.
+    assert (s: sto) by admit. assert (Wf: wf_sto s G) by admit. (* TODO as hypothesis *)
+    apply (has_to_good_bounds _ Wf) in P.
+    destruct P as [n' StB].
+    lets StA: (subtyp_tmode (subtyp_or_l Lo2 (subtyp_tmode (subtyp_refl G Lo1 n')))).
+    lets StC: (subtyp_tmode (subtyp_and_r Hi1 (subtyp_tmode (subtyp_refl G Hi2 n')))).
+    lets St: (subtyp_trans StA (subtyp_trans StB StC)).
+    (* TODO termination measure ??? *)
+    lets Q: (swap_sub_and_has_IH St Hi2Has).
+    destruct Q as [Dm [Fm [n'' [Lo1Has Sdm2]]]].
+    lets R: (swap_sub_and_has_IH St2 Lo1Has).
+    destruct R as [D1 [F1 [n''' [T1Has Sd1m]]]].
+    exists D1 (F1 \u Fm) (max n''' n'').
+    apply (conj T1Has).
+    intros x Frx.
+    assert (xF1: x \notin F1) by auto. specialize (Sd1m x xF1).
+    assert (xFm: x \notin Fm) by auto. specialize (Sdm2 x xFm).
+    lets Sdm2': (narrow_subdec_end (okadmit _) St2 Sdm2).
+    apply (subdec_trans_with_different_sizes Sd1m Sdm2').
+  + (* case subtyp_tmode *)
+    intros. apply* H0.
+  + (* case subtyp_trans *)
+    introv St12 IH12 St23 IH23 T3Has. rename D2 into D3.
+    specialize (IH23 _ _ T3Has). destruct IH23 as [D2 [L23 [n23 [T2Has Sd23]]]].
+    specialize (IH12 _ _ T2Has). destruct IH12 as [D1 [L12 [n12 [T1Has Sd12]]]].
+    exists D1 (L12 \u L23) (max n12 n23). apply (conj T1Has).
+    intros x N.
+    assert (xL12: x \notin L12) by auto. specialize (Sd12 x xL12).
+    assert (xL23: x \notin L23) by auto. specialize (Sd23 x xL23).
+    lets Sd23': (narrow_subdec_end (okadmit _) St12 Sd23).
+    apply (subdec_trans_with_different_sizes Sd12 Sd23').
+  + (* case subtyp_and *)
+    intros G T U V n StU IHU StV IHV l D2 UVHas.
+    apply invert_typ_and_has in UVHas. destruct UVHas as [UHas | [VHas | UVHas]].
+    - apply* IHU.
+    - apply* IHV.
+    - destruct UVHas as [D2U [D2V [UHas [VHas Eq]]]]. subst.
+      specialize (IHU _ _ UHas). destruct IHU as [D1U [LU [nU [THasD1U SdU]]]].
+      specialize (IHV _ _ VHas). destruct IHV as [D1V [LV [nV [THasD1V SdV]]]].
+      exists (intersect_dec D1U D1V) (LU \u LV) (max nU nV).
+      apply (conj (intersect_typ_has THasD1U THasD1V)).
+      intros x Frx.
+      assert (xLU: x \notin LU) by auto. specialize (SdU x xLU).
+      assert (xLV: x \notin LV) by auto. specialize (SdV x xLV).
+      admit. (* TODO follows from SdU and SdV *)
+  + (* case subtyp_and_l *)
+    intros G U V T n St IH l D2 THas.
+    specialize (IH _ _ THas). destruct IH as [D1U [L [n' [UHas Sd]]]].
+    exists D1U L n'. split.
+    - apply (typ_and_has_1 _ UHas).
+    - intros x xL. specialize (Sd x xL).
+      lets St': (subtyp_tmode (subtyp_and_l V (subtyp_tmode (subtyp_refl G U 0)))).
+      apply (narrow_subdec_end (okadmit _) St' Sd).
+  + (* case subtyp_and_r *)
+    intros G U V T n St IH l D2 THas.
+    specialize (IH _ _ THas). destruct IH as [D1V [L [n' [VHas Sd]]]].
+    exists D1V L n'. split.
+    - apply (typ_and_has_2 _ VHas).
+    - intros x xL. specialize (Sd x xL).
+      lets St': (subtyp_tmode (subtyp_and_r U (subtyp_tmode (subtyp_refl G V 0)))).
+      apply (narrow_subdec_end (okadmit _) St' Sd).
+  + (* case subtyp_or *)
+    intros G U V T n StU IHU StV IHV l D2 THas.
+    specialize (IHU _ _ THas). destruct IHU as [DU [LU [nU [UHas SdU]]]].
+    specialize (IHV _ _ THas). destruct IHV as [DV [LV [nV [VHas SdV]]]].
+    exists (union_dec DU DV) (LU \u LV) (max nU nV).
+    apply (conj (union_typ_has UHas VHas)).
+    intros x Frx.
+    assert (xLU: x \notin LU) by auto. specialize (SdU x xLU).
+    assert (xLV: x \notin LV) by auto. specialize (SdV x xLV).
+    rewrite (distribute_open_dec_over_union_dec x DU DV).
+    assert (SdAnd: subdec (G & x ~ typ_or U V)
+                          (intersect_dec (open_dec x D2) (open_dec x D2))
+                          (open_dec x D2)
+                          (max nU nV)).
+    admit. (* doesn't hold because subdec_refl doesn't (need good bounds) *)
+    refine (subdec_trans _ SdAnd).
+    (*
+    apply subdec_or. doesn't match: we have intersect<:union, but want union<:intersect!
+    *)
+    admit. (*
+  + (* case subtyp_or *)
+    intros G U V T n StU IHU StV IHV l D2 THas.
+    specialize (IHU _ _ THas). destruct IHU as [DU [LU [nU [UHas SdU]]]].
+    specialize (IHV _ _ THas). destruct IHV as [DV [LV [nV [VHas SdV]]]].
+    exists (union_dec DU DV) (LU \u LV) (max nU nV).
+    apply (conj (union_typ_has UHas VHas)).
+    intros x Frx.
+    assert (xLU: x \notin LU) by auto. specialize (SdU x xLU).
+    assert (xLV: x \notin LV) by auto. specialize (SdV x xLV).
+    rewrite (distribute_open_dec_over_union_dec x DU DV).
+    (* SdU is with (x: U), but we need it with (x: (typ_or U V)),
+       but narrowing goes the other way round! 
+       Intersection types to the rescue! *)
+    lets StAndU: (subtyp_tmode (subtyp_and_l V (subtyp_tmode (subtyp_refl G U 7)))).
+    apply (narrow_subdec_end (okadmit _) StAndU) in SdU.
+    lets StAndV: (subtyp_tmode (subtyp_and_r U (subtyp_tmode (subtyp_refl G V 7)))).
+    apply (narrow_subdec_end (okadmit _) StAndV) in SdV.
+    assert (StAndOr: subtyp oktrans G (typ_and U V) (typ_or U V) 7). {
+      apply subtyp_tmode. apply subtyp_or_l. exact StAndU.
+    }
+    (* doesn't help, still the wrong way!
+    apply (narrow_subdec_end (okadmit _) StAndOr).*)
+    apply subdec_union.
+    admit. admit. (*
+  + (* case subtyp_or *)
+    intros G U V T n StU IHU StV IHV l D2 THas.
+    (* only use left side (U) *)
+    specialize (IHU _ _ THas). destruct IHU as [DU [LU [nU [UHas SdU]]]].
+    exists DU LU nU. split.
+    - apply typ_or_has.*)
+  *)
+  + (* case subtyp_or_l *)
+    admit.
+  + (* case subtyp_or_r *)
+    admit.
+Qed.
+
+
+(* whenever we put an (x:T) binding into G, we ensure that x is not in fv(T),
+   so if we have "G |- T has (L: Lo..Hi)", Lo and Hi don't contain x either,
+   so we can shrink G until just before x, and Lo/Hi are still wf,
+   so invoke swap_sub_and_has with this smaller G *)
+
+Lemma has_sound: forall s G x ds T2 D2,
+  wf_sto s G ->
+  binds x ds s ->
+  ty_trm G (trm_var (avar_f x)) T2 ->
+  typ_has G T2 D2 ->
+  exists T1 D1,
+    ty_defs G ds T1 /\
+    typ_has G T1 D1 /\
+    subdec G D1 D2.
+Proof.
+  introv Wf Bis Tyx THas.
+  destruct (invert_wf_sto_with_sbsm Wf Bis Tyx) as [X1 [St Tyds]].
+  lets P: (swap_sub_and_has St X2Has).
+          (*************************)
+  destruct P as [D1 [L [n' [X1Has Sd]]]].
+  pick_fresh z. assert (zL: z \notin L) by auto. specialize (Sd z zL).
+  exists X1 D1 n'.
+  refine (conj Tyds (conj X1Has _)).
+  (* close enough ;-) [need some substitution...]
+
+  lets BiG: (sto_binds_to_ctx_binds Wf Bis).
+  lets Tyx1: (ty_var BiG).
+  lets Ok: (wf_sto_to_ok_G Wf).
+  assert (Ok': ok (G & z ~ typ_bind Ds1)) by auto.
+  lets Sds': (@subdecs_subst_principle _ z x (typ_bind Ds1)
+              (***********************) (open_decs z Ds1) (open_decs z Ds2) Ok' Sds Tyx1).
+  assert (zDs1: z \notin fv_decs Ds1) by auto.
+  assert (zDs2: z \notin fv_decs Ds2) by auto.
+  rewrite <- (@subst_intro_decs z x Ds1 zDs1) in Sds'.
+  rewrite <- (@subst_intro_decs z x Ds2 zDs2) in Sds'.
+  apply (decs_has_open x) in Ds2Has.
+  destruct (decs_has_preserves_sub Ds2Has Sds') as [D1 [Ds1Has Sd]].
+  exists Ds1 D1.
+  apply (conj Tyds (conj Ds1Has Sd)).
+  *)
+Admitted.
+
+Print Assumptions has_sound.
+*)
+
+(*
+Lemma ty_open_defs_change_var: forall x y G ds Ds S,
+  ok (G & x ~ S) ->
+  ok (G & y ~ S) ->
+  x \notin fv_defs ds ->
+  x \notin fv_decs Ds ->
+  ty_defs (G & x ~ S) (open_defs x ds) (open_decs x Ds) ->
+  ty_defs (G & y ~ S) (open_defs y ds) (open_decs y Ds).
+Proof.
+  introv Okx Oky Frds FrDs Ty.
+  destruct (classicT (x = y)) as [Eq | Ne].
+  + subst. assumption.
+  + assert (Okyx: ok (G & y ~ S & x ~ S)) by destruct* (ok_push_inv Okx).
+    assert (Ty': ty_defs (G & y ~ S & x ~ S) (open_defs x ds) (open_decs x Ds))
+      by apply (weaken_ty_defs_middle Ty Okyx).
+    rewrite* (@subst_intro_defs x y ds).
+    rewrite* (@subst_intro_decs x y Ds).
+    lets Tyy: (ty_var (binds_push_eq y S G)).
+    destruct (subst_principles y S) as [_ [_ [_ [_ [_ [_ [_ P]]]]]]].
+             (****************)
+    specialize (P _ _ _ Ty' (G & y ~ S) empty x).
+    rewrite concat_empty_r in P.
+    specialize (P eq_refl Tyy Okyx).
+    unfold subst_ctx in P. rewrite map_empty in P. rewrite concat_empty_r in P.
+    exact P.
+Qed.
+*)
+
+(* ###################################################################### *)
+(** ** Progress *)
+
+Theorem progress_result: progress.
+Proof.
+  introv Wf Ty. gen G e T Ty s Wf.
+  introv Ty. induction Ty.
+  + (* case ty_var *)
+    rename H into BiG. introv Wf.
+    right. destruct (ctx_binds_to_sto_binds Wf BiG) as [o Bis].
+    exists x o. auto.
+  + (* case ty_sel *)
+    rename H into THas. introv Wf.
+    left. specialize (IHTy s Wf). destruct IHTy as [IH | IH].
+    (* receiver is an expression *)
+    - destruct IH as [s' [e' IH]]. do 2 eexists. apply (red_sel1 l IH).
+    (* receiver is a var *)
+    - destruct IH as [x [ds [Eq Bis]]]. subst.
+      lets P: (has_sound Wf Bis Has).
+              (*********)
+      destruct P as [T1 [D1 [n [Tyds [THas Sd]]]]].
+      lets Q: (invert_ty_defs Tyds THas).
+              (**************)
+      destruct Q as [d [D0 [n0 [dsHas [Tyd Sd']]]]].
+      assert (exists T0 r, d = (def_fld T0 r)) by admit. (* <------ TODO *)
+      destruct H as [T0 [r Eq]]. subst d.
+      exists (trm_var r) s.
+      apply (red_sel Bis dsHas).
+  (* case ty_call *)
+  + intros G t m U V u Has IHrec Tyu IHarg s Wf. left.
+    specialize (IHrec s Wf eq_refl). destruct IHrec as [IHrec | IHrec].
+    - (* case receiver is an expression *)
+      destruct IHrec as [s' [e' IHrec]]. do 2 eexists. apply (red_call1 m _ IHrec).
+    - (* case receiver is  a var *)
+      destruct IHrec as [x [[Tds ds] [Eq Bis]]]. subst.
+      specialize (IHarg s Wf). destruct IHarg as [IHarg | IHarg].
+      * (* arg is an expression *)
+        destruct IHarg as [s' [e' IHarg]]. do 2 eexists. apply (red_call2 x m IHarg).
+      * (* arg is a var *)
+        destruct IHarg as [y [o [Eq Bisy]]]. subst.
+        lets P: (has_sound Wf Bis Has).
+                (*********)
+        destruct P as [Ds1 [D1 [Tyds [Ds1Has Sd]]]].
+        destruct (decs_has_to_defs_has Tyds Ds1Has) as [d dsHas].
+        destruct (defs_has_mtd_sync dsHas) as [body Eqd]. subst.
+        exists (open_trm y body) s.
+        apply (red_call y Bis dsHas).
+  (* case ty_new *)
+  + intros L G ds Ds Tyds F s Wf.
+    left. pick_fresh x.
+    exists (trm_var (avar_f x)) (s & x ~ (object Ds ds)).
+    apply* red_new.
+  (* case ty_sbsm *)
+  + intros. auto_specialize. assumption.
+Qed.
+
+Print Assumptions progress_result.
+
+
+(* ###################################################################### *)
+(** ** Preservation *)
+
+Theorem preservation_proof:
+  forall e s e' s' (Hred: red e s e' s') G T (Hwf: wf_sto s G) (Hty: ty_trm G e T),
+  exists H, wf_sto s' (G & H) /\ ty_trm (G & H) e' T.
+Proof.
+  intros s e s' e' Red. induction Red.
+  (* red_call *)
+  + intros G U3 Wf TyCall. rename H into Bis, H0 into dsHas, T into X1.
+    exists (@empty typ). rewrite concat_empty_r. apply (conj Wf).
+    apply invert_ty_call in TyCall.
+    destruct TyCall as [T2 [U2 [Has [StU23 Tyy]]]].
+    lets P: (has_sound Wf Bis Has).
+            (*********)
+    destruct P as [Ds1 [D1 [Tyds [Ds1Has Sd]]]].
+    apply invert_subdec_mtd_sync_left in Sd.
+    destruct Sd as [T1 [U1 [Eq [StT StU12]]]]. subst D1.
+    destruct (invert_ty_mtd_inside_ty_defs Tyds dsHas Ds1Has) as [L0 Tybody].
+    apply invert_ty_var in Tyy.
+    destruct Tyy as [T3 [StT3 Biy]].
+    pick_fresh y'.
+    rewrite* (@subst_intro_trm y' y body).
+    assert (Fry': y' \notin fv_typ U3) by auto.
+    assert (Eqsubst: (subst_typ y' y U3) = U3)
+      by apply* subst_fresh_typ_dec_decs.
+    rewrite <- Eqsubst.
+    lets Ok: (wf_sto_to_ok_G Wf).
+    apply (@trm_subst_principle G y' y (open_trm y' body) T1 _).
+           (*******************)
+    - auto.
+    - assert (y'L0: y' \notin L0) by auto. specialize (Tybody y' y'L0).
+      apply (ty_sbsm Tybody).
+      apply weaken_subtyp_end. auto. apply (subtyp_trans StU12 StU23).
+    - refine (ty_sbsm _ StT). refine (ty_sbsm _ StT3). apply (ty_var Biy).
+  (* red_sel *)
+  + intros G T3 Wf TySel. rename H into Bis, H0 into dsHas.
+    exists (@empty typ). rewrite concat_empty_r. apply (conj Wf).
+    apply invert_ty_sel in TySel.
+    destruct TySel as [T2 [StT23 Has]].
+    lets P: (has_sound Wf Bis Has).
+            (*********)
+    destruct P as [Ds1 [D1 [Tyds [Ds1Has Sd]]]].
+    apply invert_subdec_fld_sync_left in Sd.
+    destruct Sd as [T1 [Eq StT12]]. subst D1.
+    refine (ty_sbsm _ StT23).
+    refine (ty_sbsm _ StT12).
+    apply (invert_ty_fld_inside_ty_defs Tyds dsHas Ds1Has).
+  (* red_new *)
+  + rename T into Ds1. intros G T2 Wf Ty.
+    apply invert_ty_new in Ty.
+    destruct Ty as [StT12 [L [Tyds Cb]]].
+    exists (x ~ (typ_bind Ds1)).
+    pick_fresh x'. assert (Frx': x' \notin L) by auto.
+    specialize (Tyds x' Frx').
+    assert (xG: x # G) by apply* sto_unbound_to_ctx_unbound.
+    split.
+    - apply (wf_sto_push _ Wf H xG).
+      * apply* (@ty_open_defs_change_var x').
+      * exact Cb. (* was a "meh TODO" before cbounds :-) *)
+    - lets Ok: (wf_sto_to_ok_G Wf). assert (Okx: ok (G & x ~ (typ_bind Ds1))) by auto.
+      apply (weaken_subtyp_end Okx) in StT12.
+      refine (ty_sbsm _ StT12). apply ty_var. apply binds_push_eq.
+  (* red_call1 *)
+  + intros G Tr2 Wf TyCall.
+    apply invert_ty_call in TyCall.
+    destruct TyCall as [Ta [Tr1 [Has [St Tya]]]].
+    apply invert_has in Has.
+    destruct Has as [Has | Has].
+    - (* case has_trm *)
+      destruct Has as [To [Ds [Tyo [Exp [DsHas Clo]]]]].
+      specialize (IHRed G To Wf Tyo). destruct IHRed as [H [Wf' Tyo']].
+      lets Ok: (wf_sto_to_ok_G Wf').
+      exists H. apply (conj Wf').
+      apply (weaken_subtyp_end Ok) in St.
+      refine (ty_sbsm _ St).
+      apply (@ty_call (G & H) o' m Ta Tr1 a).
+      * refine (has_trm Tyo' _ DsHas Clo).
+        apply (weaken_exp_end Ok Exp).
+      * apply (weaken_ty_trm_end Ok Tya).
+    - (* case has_var *)
+      destruct Has as [x [Tx [Ds [D' [Eqx _]]]]]. subst.
+      inversion Red. (* contradiction: vars don't step *)
+  (* red_call2 *)
+  + intros G Tr2 Wf TyCall.
+    apply invert_ty_call in TyCall.
+    destruct TyCall as [Ta [Tr1 [Has [St Tya]]]].
+    specialize (IHRed G Ta Wf Tya).
+    destruct IHRed as [H [Wf' Tya']].
+    exists H. apply (conj Wf').
+    lets Ok: wf_sto_to_ok_G Wf'.
+    apply (weaken_subtyp_end Ok) in St.
+    refine (ty_sbsm _ St).
+    apply (@ty_call (G & H) _ m Ta Tr1 a').
+    - apply (weaken_has_end Ok Has).
+    - assumption.
+  (* red_sel1 *)
+  + intros G T2 Wf TySel.
+    apply invert_ty_sel in TySel.
+    destruct TySel as [T1 [St Has]].
+    apply invert_has in Has.
+    destruct Has as [Has | Has].
+    - (* case has_trm *)
+      destruct Has as [To [Ds [Tyo [Exp [DsHas Clo]]]]].
+      specialize (IHRed G To Wf Tyo). destruct IHRed as [H [Wf' Tyo']].
+      lets Ok: (wf_sto_to_ok_G Wf').
+      exists H. apply (conj Wf').
+      apply (weaken_subtyp_end Ok) in St.
+      refine (ty_sbsm _ St). apply (@ty_sel (G & H) o' l T1).
+      refine (has_trm Tyo' _ DsHas Clo).
+      apply (weaken_exp_end Ok Exp).
+    - (* case has_var *)
+      destruct Has as [x [Tx [Ds [D' [Eqx _]]]]]. subst.
+      inversion Red. (* contradiction: vars don't step *)
+Qed.
+
+Theorem preservation_result: preservation.
+Proof.
+  introv Hwf Hty Hred.
+  destruct (preservation_proof Hred Hwf Hty) as [H [Hwf' Hty']].
+  exists (G & H). split; assumption.
+Qed.
+
+Print Assumptions preservation_result.
